progress on eval version

theories_unscoped/LevelTwo.v
@@ -1,10 +1,20 @@
-From Prototype Require Import Prelude Sig.
+From Prototype Require Import Prelude Sig LevelOne.
 
 Module Make (S : Sig).
+Module O := LevelOne.Make (S).
 Definition arg_ty := @arg_ty (base S.t).
 
 (*********************************************************************************)
-(** *** Expressions (terms and substitutions). *)
+(** *** Explicit renamings. *)
+(*********************************************************************************)
+
+(** Notations for common renamings. *)
+Notation "'↑ᵣ' k" := (R_shift k) (at level 0, k at level 0).
+Notation "i '.ᵣ' r" := (R_cons i r) (at level 60, right associativity).
+Notation "r1 '>>ᵣ' r2" := (R_comp r1 r2) (at level 50, left associativity).
+
+(*********************************************************************************)
+(** *** Expressions (terms and explicit substitutions). *)
 (*********************************************************************************)
 
 (** Kind of a term, argument, or argument list. *)
@@ -17,18 +27,25 @@ Inductive mono_kind :=
   Kal : list arg_ty -> mono_kind.
 Derive NoConfusion for mono_kind.
 
+(** Kind of a renaming or substitution. *)
+Inductive ren_kind :=
+| (** *)
+
 (** Expressions are indexed by kinds. *)
 Inductive kind : Type := 
-| (** Term, argument, or argument list. *)
+| (** Term-like. *)
   Km : mono_kind -> kind
-| (** Substitution. *)
-  Ks : kind.  
+| (** Substitution-like. *)
+  Kb : bi_kind -> kind.  
 Derive NoConfusion for kind.
 
-(** An expression metavariable is encoded as a unique identifier (a natural).
-    When denoting a expr, we have access to an environment which maps metavariable identifiers
-    to actual (denoted) expressions. *)
-Definition mvar (k : kind) := nat.
+Definition denote_type (k : kind) : Type :=
+  match k with 
+  | Km Kt => O.expr O.Kt
+  | Km (Kal tys) => O.expr (O.Kal tys)
+  | Km (Ka ty) => O.expr (O.Ka ty)
+  | Ks => O.subst
+  end.
 
 (** Notations for expressions with known kinds. *)
 Reserved Notation "'term'" (at level 0).
@@ -40,48 +57,71 @@ Reserved Notation "'subst'" (at level 0).
     Expressions are indexed by a kind: this is to avoid writing a mutual inductives,
     which would be hard to manipulate. *)
 Inductive expr : kind -> Type :=
-| (** Term variable. *)
-  E_var : nat -> term
+| (** Variable term constructor (de Bruijn index). *)
+  T_var : nat -> term
 | (** Non-variable term constructor, applied to a list of arguments. *)
-  E_ctor : forall c, args (ctor_type S.t c) -> term
+  T_ctor : forall c, args (ctor_type S.t c) -> term
+
 | (** Empty argument list. *)
-  E_al_nil : args []
+  AL_nil : args []
 | (** Non-empty argument list. *)
-  E_al_cons {ty tys} : arg ty -> args tys -> args (ty :: tys)
+  AL_cons {ty tys} : arg ty -> args tys -> args (ty :: tys)
+
 | (** Base argument (e.g. bool or string). *)
-  E_abase : forall b, denote_base S.t b -> arg (AT_base b)
+  A_base : forall b, denote_base S.t b -> arg (AT_base b)
 | (** Term argument. *)
-  E_aterm : term -> arg AT_term
+  A_term : term -> arg AT_term
 | (** Binder argument. *)
-  E_abind {ty} : arg ty -> arg (AT_bind ty)
-| (** Substitution applied to a term/argument/argument-list. *)
-  E_subst {k} : expr (Km k) -> subst -> expr (Km k)
+  A_bind {ty} : arg ty -> arg (AT_bind ty)
+
+| (** Shift renaming. *)
+  R_shift : nat -> ren
+| (** Renaming expansion. *)
+  R_cons : nat -> ren -> ren
+| (** Renaming composition. *)
+  R_comp : ren -> ren -> ren
+
 | (** Shift substitution. *)
-  E_sshift : nat -> subst
+  S_shift : nat -> subst
 | (** Substitution expansion. *)
-  E_scons : term -> subst -> subst
+  S_cons : term -> subst -> subst
 | (** Substitution composition. *)
-  E_scomp : subst -> subst -> subst
-| (** Metavariable. *)
-  E_mvar {k} : mvar k -> expr k
+  S_comp : subst -> subst -> subst
+| (** View a renaming as a substitution. *)
+  S_ren : ren -> subst
+
+| (** Instantiate a term/argument/argument-list with a renaming. *)
+  E_rinst {k} : expr (Km k) -> ren -> expr (Km k)
+| (** Metavariable (of any kind). *)
+  E_mvar {k} : denote_type k -> expr k
+
 where "'term'" := (expr (Km Kt))
   and "'arg' ty" := (expr (Km (Ka ty)))
   and "'args' tys" := (expr (Km (Kal tys)))
   and "'subst'" := (expr Ks).
+
 Derive Signature NoConfusion for expr.
 
 (** Notations for common expressions. *)
-Notation "↑ k" := (E_sshift k) (at level 0, k at level 0).
-Notation "t .: s" := (E_scons t s) (at level 60, right associativity).
-Notation "s1 >> s2" := (E_scomp s1 s2) (at level 50, left associativity).
-Notation "t '[:' s ']'" := (E_subst t s) (at level 15, s at level 0, no associativity).
+
+Notation "'↑ₛ' k" := (S_shift k) (at level 0, k at level 0).
+Notation "t '.ₛ' s" := (S_cons t s) (at level 60, right associativity).
+Notation "s1 '>>ₛ' s2" := (S_comp s1 s2) (at level 50, left associativity).
+Notation "t '[:' s ']'" := (E_inst t s) (at level 15, s at level 0, no associativity).
+
+(** The identity renaming. *)
+Definition rid : ren := R_shift 0.
 
 (** The identity substitution. *)
-Definition sid : subst := E_sshift 0.
+Definition sid : subst := S_shift 0.
+
+(** Lift a renaming through a binder. *)
+Definition up_ren (r : ren) : ren :=
+  0 .ᵣ r >>ᵣ ↑ᵣ1.
 
 (** Lift a substitution through a binder. *)
-Equations up_subst (s : subst) : subst :=
-up_subst s := E_var 0 .: s >> ↑1.
+Definition up_subst (s : subst) : subst :=
+  E_var 0 .ₛ s >>ₛ ↑ₛ1.
 
 (*********************************************************************************)
 (** *** Axiomatic equality. *)
@@ -89,7 +129,7 @@ up_subst s := E_var 0 .: s >> ↑1.
 
 (** [e =σ e'] means that the expressions [e] and [e'] are equal 
     modulo the equational theory of sigma calculus. *)
-Reserved Notation "t1 '=σ' t2" (at level 75, no associativity).
+(*Reserved Notation "t1 '=σ' t2" (at level 75, no associativity).
 Inductive axiom_eq : forall {k}, expr k -> expr k -> Prop :=
 
 (** Equivalence. *)
@@ -108,66 +148,104 @@ Inductive axiom_eq : forall {k}, expr k -> expr k -> Prop :=
     t1 =σ t2 -> E_aterm t1 =σ E_aterm t2
 | aeq_congr_abind {ty} (a1 a2 : arg ty) : 
     a1 =σ a2 -> E_abind a1 =σ E_abind a2
-| aeq_congr_subst {k} (t1 t2 : expr (Km k)) (s1 s2 : subst) : 
+| aeq_congr_inst {k} (t1 t2 : expr (Km k)) (s1 s2 : subst) : 
     t1 =σ t2 -> s1 =σ s2 -> t1[: s1 ] =σ t2[: s2 ] 
 | aeq_congr_scons (t1 t2 : term) (s1 s2 : subst) : 
-    t1 =σ t2 -> s1 =σ s2 -> t1 .: s1 =σ t2 .: s2
-| aeq_congr_scomp (s1 s2 s1' s2' : subst) : 
+    t1 =σ t2 -> s1 =σ s2 -> t1 .ₛ s1 =σ t2 .ₛ s2
+| aeq_congr_comp {k1 k2} (s1 s2 : expr (K2 k1)) (s1' s2' : expr (K2 k2)) : 
     s1 =σ s2 -> s1' =σ s2' -> s1 >> s1' =σ s2 >> s2'
+
+(** Apply a renaming to a variable. *)
+
+| aeq_rshift_var i k : 
+    (E_var i)[ᵣ ↑ᵣ k ] =σ E_var (k + i)
+| aeq_rcons_zero i (r : ren) :
+    (E_var 0)[ᵣ i .ᵣ r] =σ E_var i
+| aeq_rcons_succ i j (r : ren) :
+    (E_var (S i))[ᵣ j .ᵣ r] =σ (E_var i)[ᵣ r]
 
 (** Apply a substitution to a variable. *)
 
 | aeq_sshift_var i k : 
-    (E_var i)[: ↑k ] =σ E_var (k + i)
+    (E_var i)[ₛ ↑ₛ k ] =σ E_var (k + i)
 | aeq_scons_zero (t : term) (s : subst) :
-    (E_var 0)[: t .: s] =σ t
+    (E_var 0)[ₛ t .ₛ s] =σ t
 | aeq_scons_succ i (t : term) (s : subst) :
-    (E_var (S i))[: t .: s] =σ (E_var i)[: s]
+    (E_var (S i))[ₛ t .ₛ s] =σ (E_var i)[ₛ s]
 
-(** Apply a substitution to an expression. *)
+(** Push a renaming/substitution inside an expression. *)
 
-| aeq_subst_ctor c (al : args _) (s : subst) : 
+| aeq_inst_ctor {k} c (al : args _) (s : expr (K2 k)) : 
     (E_ctor c al)[: s ] =σ E_ctor c (al[: s ])
-| aeq_subst_al_nil (s : subst) : 
+| aeq_inst_al_nil {k} (s : expr (K2 k)) : 
     E_al_nil[: s ] =σ E_al_nil
-| aeq_subst_al_cons {ty tys} (a : arg ty) (al : args tys) (s : subst) : 
+| aeq_inst_al_cons {k ty tys} (a : arg ty) (al : args tys) (s : expr (K2 k)) : 
     (E_al_cons a al)[: s ] =σ E_al_cons (a[: s]) (al[: s ])
-| aeq_subst_abase b x (s : subst) : 
+| aeq_inst_abase {k} b x (s : expr (K2 k)) : 
     (E_abase b x)[: s ] =σ E_abase b x
-| aeq_subst_aterm (t : term) (s : subst) : 
+| aeq_inst_aterm {k} (t : term) (s : expr (K2 k)) : 
     (E_aterm t)[: s ] =σ E_aterm (t[: s ])
-| aeq_subst_abind {ty} (a : arg ty) (s : subst) : 
-    (E_abind a)[: s ] =σ E_abind (a[: up_subst s ])
-| aeq_subst_subst {k} (e : expr (Km k)) (s1 s2 : subst) :
+| aeq_inst_abind_s {ty} (a : arg ty) (s : subst) : 
+    (E_abind a)[ₛ s ] =σ E_abind (a[ₛ up_subst s ])
+| aeq_inst_abind_r {ty} (a : arg ty) (r : ren) : 
+    (E_abind a)[ᵣ r ] =σ E_abind (a[ᵣ up_ren r ])
+| aeq_inst_inst {k k' k''} (e : expr (K1 k)) (s1 : expr (K2 k')) (s2 : expr (K2 k'')) :
     e[: s1 ][: s2 ] =σ e[: s1 >> s2 ]
-| aeq_subst_mvar {k} (v : mvar (Km k)) :
-    (E_mvar v)[: sid ] =σ E_mvar v 
+
+(** Renaming laws. *)
+
+| aeq_rshift_succ_r k : 
+    ↑ᵣ k >> ↑ᵣ 1 =σ ↑ᵣ (S k)
+| aeq_rshift_rcons :
+    0 .ᵣ ↑ᵣ 1 =σ ↑ᵣ 0  
+| aeq_rcons_rshift i (r : ren) :
+    ↑ᵣ 1 >> (i .ᵣ r) =σ r
+| aeq_rid_l (r : ren) : 
+    rid >> r =σ r 
+| aeq_rid_r (r : ren) : 
+    r >> rid =σ r
+| aeq_distrib_ren_subst i (r1 : ren) (s2 : subst) : 
+    (i .ᵣ r1) >> s2 =σ (E_var i)[ₛ s2 ] .ₛ r1 >> s2
+| aeq_rid_mvar {k} (v : denote_type (K1 k)) :
+    (E_mvar v)[ᵣ rid ] =σ E_mvar v 
 
 (** Substitution laws. *)
 
 | aeq_sshift_succ_r k : 
-    ↑k >> ↑1 =σ ↑(S k)
+    ↑ₛ k >> ↑ₛ 1 =σ ↑ₛ (S k)
 | aeq_sshift_scons :
-    E_var 0 .: ↑1 =σ ↑0  
+    E_var 0 .ₛ ↑ₛ 1 =σ ↑ₛ 0  
 | aeq_scons_sshift (t : term) (s : subst) :
-  ↑1 >> (t .: s) =σ s
+    ↑ₛ 1 >> (t .ₛ s) =σ s
 | aeq_sid_l (s : subst) : 
     sid >> s =σ s 
 | aeq_sid_r (s : subst) : 
     s >> sid =σ s
-| aeq_assoc (s1 s2 s3 : subst) : 
+| aeq_distrib_subst {k} (t : term) (s1 : subst) (s2 : expr (K2 k)) : 
+    (t .ₛ s1) >> s2 =σ t[: s2 ] .ₛ s1 >> s2
+| aeq_sid_mvar {k} (v : denote_type (K1 k)) :
+    (E_mvar v)[ₛ sid ] =σ E_mvar v 
+
+(** Link between substitutions and renamings. *)
+
+| aeq_ren_subst {k} (t : expr (K1 k)) (r : ren) :
+    t [ᵣ r ] =σ t [ₛ r >> sid ]
+| aeq_rshift_shift_l i : 
+    ↑ᵣ i >> sid =σ ↑ₛ i 
+| aeq_rshift_shift_r i : 
+    sid >> ↑ᵣ i =σ ↑ₛ i 
+
+| aeq_assoc {k k' k''} (s1 : expr (K2 k)) (s2 : expr (K2 k')) (s3 : expr (K2 k'')) : 
     s1 >> (s2 >> s3) =σ (s1 >> s2) >> s3
-| aeq_distrib (t : term) (s1 s2 : subst) : 
-    (t .: s1) >> s2 =σ t[: s2 ] .: s1 >> s2
 
 where "t1 '=σ' t2" := (axiom_eq t1 t2).
-Hint Constructors axiom_eq : core.
+Hint Constructors axiom_eq : core.*)
 
 (*********************************************************************************)
 (** *** Setoid rewrite support. *)
 (*********************************************************************************)
 
-#[global] Instance axiom_eq_equiv k : Equivalence (@axiom_eq k).
+(*#[global] Instance axiom_eq_equiv k : Equivalence (@axiom_eq k).
 Proof. constructor ; eauto. Qed.
 
 #[global] Instance e_ctor_proper c : Proper (axiom_eq ==> axiom_eq) (@E_ctor c).
@@ -182,21 +260,25 @@ Proof. intros ???. apply aeq_congr_aterm ; auto. Qed.
 #[global] Instance e_abind_proper ty : Proper (axiom_eq ==> axiom_eq) (@E_abind ty).
 Proof. intros ???. apply aeq_congr_abind ; auto. Qed.
 
-#[global] Instance e_subst_proper k : Proper (axiom_eq ==> axiom_eq ==> axiom_eq) (@E_subst k).
-Proof. intros ??????. apply aeq_congr_subst ; auto. Qed.
+#[global] Instance e_inst_proper k1 k2 : Proper (axiom_eq ==> axiom_eq ==> axiom_eq) (@E_inst k1 k2).
+Proof. intros ??????. apply aeq_congr_inst ; auto. Qed.
 
 #[global] Instance e_scons_proper : Proper (axiom_eq ==> axiom_eq ==> axiom_eq) E_scons.
 Proof. intros ??????. apply aeq_congr_scons ; auto. Qed.
 
-#[global] Instance e_scomp_proper : Proper (axiom_eq ==> axiom_eq ==> axiom_eq) E_scomp.
-Proof. intros ??????. apply aeq_congr_scomp ; auto. Qed.
+#[global] Instance e_comp_proper k1 k2 : Proper (axiom_eq ==> axiom_eq ==> axiom_eq) (@E_comp k1 k2).
+Proof. intros ??????. apply aeq_congr_comp ; auto. Qed.*)
 
 (*********************************************************************************)
 (** *** Additional functions and properties. *)
 (*********************************************************************************)
 
-Lemma up_subst_sid : up_subst sid =σ sid.
-Proof. autorewrite with up_subst. rewrite aeq_sid_l. now rewrite aeq_sshift_scons. Qed.
+(*Lemma up_subst_sid : up_subst sid =σ sid.
+Proof. unfold up_subst. rewrite aeq_sid_l. now rewrite aeq_sshift_scons. Qed.
+
+Lemma up_ren_rid : up_ren rid =σ rid.
+Proof. unfold up_ren. rewrite aeq_rid_l. now rewrite aeq_sshift_scons. Qed.
+
 
 Lemma aeq_sshift_succ_l k : ↑1 >> ↑k =σ ↑(S k).
 Proof. 
@@ -230,6 +312,9 @@ dependent induction e ; auto.
 - now rewrite aeq_subst_aterm, IHe.
 - now rewrite aeq_subst_abind, up_subst_sid, IHe.
 - rewrite aeq_subst_subst. now rewrite aeq_sid_r.
-Qed.
+Qed.*)
+
+
+
 
 End Make.
