theories_eval/LevelTwo.v
@@ -1,0 +1,575 @@
+From Prototype Require Import Prelude Sig LevelOne.
+
+Module Make (S : Sig).
+Module O := LevelOne.Make (S).
+Definition arg_ty := @arg_ty (base S.t).
+
+(*********************************************************************************)
+(** *** Expressions (terms and explicit substitutions). *)
+(*********************************************************************************)
+
+(** Kind of a term, argument, or argument list. *)
+Inductive mono_kind :=
+| (** Term. *)
+  Kt : mono_kind
+| (** Constructor argument. *)
+  Ka : arg_ty -> mono_kind
+| (** List of constructor arguments. *)
+  Kal : list arg_ty -> mono_kind.
+Derive NoConfusion for mono_kind.
+
+(** Kind of a renaming or substitution. *)
+Inductive bi_kind :=
+| (** Renaming *) 
+  Kr : bi_kind
+| (** Substitution. *)
+  Ks : bi_kind.
+Derive NoConfusion for bi_kind.
+
+(** Expressions are indexed by kinds. *)
+Inductive kind : Type := 
+| (** Term-like. *)
+  Km : mono_kind -> kind
+| (** Substitution-like. *)
+  Kb : bi_kind -> kind.  
+Derive NoConfusion for kind.
+
+Definition denote_type (k : kind) : Type :=
+  match k with 
+  | Km k' => 
+    (* Since [denote_type] is used in types a lot, it is important that it computes
+       as much as possible. We match on [k'] rather late so that [denote_type (Km _)]
+       is not stuck and computes to [O.expr _]. *)
+    O.expr (match k' with Kt => O.Kt | Ka ty => O.Ka ty | Kal tys => O.Kal tys end)
+  | Kb Kr => O.ren
+  | Kb Ks => O.subst
+  end.
+
+(** Notations for expressions with known kinds. *)
+Reserved Notation "'term'" (at level 0).
+Reserved Notation "'arg' ty" (at level 0, ty at level 0).
+Reserved Notation "'args' tys" (at level 0, tys at level 0).
+Reserved Notation "'ren'" (at level 0).
+Reserved Notation "'subst'" (at level 0).
+
+(** Expressions over an abstract signature. 
+    Expressions are indexed by a kind: this is to avoid writing a mutual inductives,
+    which would be hard to manipulate. *)
+Inductive expr : kind -> Type :=
+
+| (** Variable term constructor (de Bruijn index). *)
+  E_tvar : nat -> term
+| (** Non-variable term constructor, applied to a list of arguments. *)
+  E_tctor : forall c, args (ctor_type S.t c) -> term
+
+| (** Empty argument list. *)
+  E_al_nil : args []
+| (** Non-empty argument list. *)
+  E_al_cons {ty tys} : arg ty -> args tys -> args (ty :: tys)
+
+| (** Base argument (e.g. bool or string). *)
+  E_abase : forall b, denote_base S.t b -> arg (AT_base b)
+| (** Term argument. *)
+  E_aterm : term -> arg AT_term
+| (** Binder argument. *)
+  E_abind {ty} : arg ty -> arg (AT_bind ty)
+
+| (** Shift renaming. *)
+  E_rshift : nat -> ren
+| (** Renaming expansion. *)
+  E_rcons : nat -> ren -> ren
+| (** Renaming composition. *)
+  E_rcomp : ren -> ren -> ren
+
+| (** Shift substitution. *)
+  E_sshift : nat -> subst
+| (** Substitution expansion. *)
+  E_scons : term -> subst -> subst
+| (** Substitution composition. *)
+  E_scomp : subst -> subst -> subst
+| (** View a renaming as a substitution. *)
+  E_sren : ren -> subst
+
+| (** Instantiate a term/argument/argument-list with a renaming. *)
+  E_rinst {k} : expr (Km k) -> ren -> expr (Km k)
+| (** Instantiate a term/argument/argument-list with a substitution. *)
+  E_sinst {k} : expr (Km k) -> subst -> expr (Km k)
+| (** Metavariable (of any kind). *)
+  E_mvar {k} : denote_type k -> expr k
+
+where "'term'" := (expr (Km Kt))
+  and "'arg' ty" := (expr (Km (Ka ty)))
+  and "'args' tys" := (expr (Km (Kal tys)))
+  and "'ren'" := (expr (Kb Kr))
+  and "'subst'" := (expr (Kb Ks)).
+
+Derive Signature NoConfusion for expr.
+
+(** Notations for common expressions. *)
+
+Notation "'↑ᵣ' k" := (E_rshift k) (at level 0, k at level 0).
+Notation "i '.ᵣ' r" := (E_rcons i r) (at level 60, right associativity).
+Notation "r1 '>>ᵣ' r2" := (E_rcomp r1 r2) (at level 50, left associativity).
+
+Notation "'↑ₛ' k" := (E_sshift k) (at level 0, k at level 0).
+Notation "t '.ₛ' s" := (E_scons t s) (at level 60, right associativity).
+Notation "s1 '>>ₛ' s2" := (E_scomp s1 s2) (at level 50, left associativity).
+
+Notation "t '[ᵣ' s ']'" := (E_rinst t s) (at level 15, s at level 0, no associativity).
+Notation "t '[ₛ' s ']'" := (E_sinst t s) (at level 15, s at level 0, no associativity).
+
+(** The identity renaming. *)
+Definition rid : ren := E_rshift 0.
+
+(** The identity substitution. *)
+Definition sid : subst := E_sshift 0.
+
+(** Lift a renaming through a binder. *)
+Definition up_ren (r : ren) : ren :=
+  0 .ᵣ r >>ᵣ ↑ᵣ1.
+
+(** Lift a substitution through a binder. *)
+Definition up_subst (s : subst) : subst :=
+  E_tvar 0 .ₛ s >>ₛ ↑ₛ1.
+
+(*********************************************************************************)
+(** *** Denotation. *)
+(*********************************************************************************)
+
+(** Mapping from level two expressions to level one expressions and substitutions. *)
+Equations denote {k} (t : expr k) : denote_type k by struct t :=
+
+denote (E_tvar i) := O.E_var i ;
+denote (E_tctor c al) := O.E_ctor c (denote al) ;
+
+denote E_al_nil := O.E_al_nil ;
+denote (E_al_cons a al) := O.E_al_cons (denote a) (denote al) ;
+
+denote (E_abase b x) := O.E_abase b x ;
+denote (E_aterm t) := O.E_aterm (denote t) ;
+denote (E_abind a) := O.E_abind (denote a) ;
+
+denote (E_rshift k) := O.rshift k ;
+denote (E_rcons i r) := O.rcons i (denote r) ;
+denote (E_rcomp r1 r2) := O.rcomp (denote r1) (denote r2) ;
+
+denote (E_sshift k) := O.sshift k ;
+denote (E_scons t s) := O.scons (denote t) (denote s) ;
+denote (E_scomp s1 s2) := O.scomp (denote s1) (denote s2) ;
+denote (E_sren r) := fun i => O.E_var (denote r i) ;
+
+denote (@E_sinst Kt t s) := O.substitute (denote t) (denote s) ;
+denote (@E_sinst (Ka _) t s) := O.substitute (denote t) (denote s) ;
+denote (@E_sinst (Kal _) t s) := O.substitute (denote t) (denote s) ;
+denote (@E_rinst Kt t s) := O.rename (denote t) (denote s) ;
+denote (@E_rinst (Ka _) t s) := O.rename (denote t) (denote s) ;
+denote (@E_rinst (Kal _) t s) := O.rename (denote t) (denote s) ;
+denote (E_mvar x) := x.
+
+(*********************************************************************************)
+(** *** Reification. *)
+(*********************************************************************************)
+
+Ltac2 rec reify_term (t : constr) : constr :=
+  lazy_match! t with 
+  | O.E_var ?i => constr:(E_tvar $i)
+  | O.E_ctor ?c ?al => 
+    let al := reify_term al in
+    constr:(E_tctor $c $al)
+  | O.E_al_nil => constr:(E_al_nil)
+  | O.E_al_cons ?a ?al => 
+    let a := reify_term a in
+    let al := reify_term al in
+    constr:(E_al_cons $a $al)
+  | O.E_abase ?b ?x => constr:(E_abase $b $x)
+  | O.E_aterm ?t => 
+    let t := reify_term t in
+    constr:(E_aterm $t)
+  | O.E_abind ?a =>
+    let a := reify_term a in
+    constr:(E_abind $a)
+  | O.rename ?t ?r =>
+    let t := reify_term t in
+    let r := reify_ren r in
+    constr:(E_rinst $t $r)
+  | O.substitute ?t ?s =>
+    let t := reify_term t in
+    let s := reify_subst s in
+    constr:(E_sinst $t $s)
+  | _ => constr:(@E_mvar (Km Kt) $t)
+  end
+with reify_subst (s : constr) : constr :=
+  lazy_match! s with 
+  | O.sid => constr:(sid)
+  | O.sshift ?k => constr:(E_sshift $k)
+  | O.scons ?t ?s =>
+    let t := reify_term t in 
+    let s := reify_subst s in 
+    constr:(E_scons $t $s)
+  | O.scomp ?s1 ?s2 =>
+    let s1 := reify_subst s1 in 
+    let s2 := reify_subst s2 in 
+    constr:(E_scomp $s1 $s2)
+  | fun i => O.rename (?s i) ?r =>
+    let s := reify_subst s in 
+    let r := reify_ren r in
+    constr:(E_scomp $s (E_sren $r))
+  | ?s => constr:(@E_mvar (Kb Ks) $s)
+  end
+with reify_ren (r : constr) : constr := 
+  lazy_match! r with 
+  | O.rid => constr:(rid)
+  | O.rshift ?k => constr:(E_rshift $k)
+  | O.rcons ?i ?r => 
+    let r := reify_ren r in 
+    constr:(E_rcons $i $r)
+  | ?r => constr:(@E_mvar (Kb Kr) $r)
+  end.
+
+(*********************************************************************************)
+(** *** Normal form expressions. *)
+(*********************************************************************************)
+
+Reserved Notation "'nf_term'" (at level 0).
+Reserved Notation "'nf_arg' ty" (at level 0, ty at level 0).
+Reserved Notation "'nf_args' tys" (at level 0, tys at level 0).
+Reserved Notation "'nf_ren'" (at level 0).
+Reserved Notation "'nf_subst'" (at level 0).
+
+(** Normal form expressions. *)
+Inductive nf_expr : kind -> Type :=
+
+| N_tvar : nat -> nf_term
+| N_tctor : forall c, nf_args (ctor_type S.t c) -> nf_term
+| N_al_nil : nf_args []
+| N_al_cons {ty tys} : nf_arg ty -> nf_args tys -> nf_args (ty :: tys)
+| N_abase : forall b, denote_base S.t b -> nf_arg (AT_base b)
+| N_aterm : nf_term -> nf_arg AT_term
+| N_abind {ty} : nf_arg ty -> nf_arg (AT_bind ty)
+
+| N_rshift : nat -> nf_ren
+| N_rcons : nat -> nf_ren -> nf_ren
+(** Composition of renamings, where the left hand side is a 
+    (possibly lifted) metavariable. *)
+|  N_rcomp : nat -> denote_type (Kb Kr) -> nf_ren -> nf_ren
+
+| N_sshift : nat -> nf_subst
+| N_scons : nf_term -> nf_subst -> nf_subst
+(** Composition of substitutions, where the left hand side is a 
+    (possibly lifted) metavariable. *)
+| N_scomp : nat -> denote_type (Kb Ks) -> nf_subst -> nf_subst
+| N_sren : nf_ren -> nf_subst
+
+(** Instantiation with a renaming/substitution, where the left hand side 
+    is a metavariable. *)  
+| N_rinst_l {k} : denote_type (Km k) -> nf_ren -> nf_expr (Km k)
+| N_sinst_l {k} : denote_type (Km k) -> nf_subst -> nf_expr (Km k)
+(** Instantiation with a renaming/substitution, where the right hand side 
+    is a metavariable (possibly composed with some other renaming/substitution),
+    and the left hand side is a de Bruijn index. *)
+| N_rinst_r : nat -> denote_type (Kb Kr) -> nf_ren -> nf_term
+| N_sinst_r : nat -> denote_type (Kb Ks) -> nf_subst -> nf_term
+
+where "'nf_term'" := (nf_expr (Km Kt))
+  and "'nf_arg' ty" := (nf_expr (Km (Ka ty)))
+  and "'nf_args' tys" := (nf_expr (Km (Kal tys)))
+  and "'nf_ren'" := (nf_expr (Kb Kr))
+  and "'nf_subst'" := (nf_expr (Kb Ks)).
+
+(** Denote a normal form expression. *)
+Equations denote_nf {k} : nf_expr k -> denote_type k :=
+
+denote_nf (N_tvar i) := O.E_var i ;
+denote_nf (N_tctor c al) := O.E_ctor c (denote_nf al) ;
+denote_nf N_al_nil := O.E_al_nil ;
+denote_nf (N_al_cons a al) := O.E_al_cons (denote_nf a) (denote_nf al) ;
+denote_nf (N_abase b x) := O.E_abase b x ;
+denote_nf (N_aterm t) := O.E_aterm (denote_nf t) ;
+denote_nf (N_abind a) := O.E_abind (denote_nf a) ;
+
+denote_nf (N_rshift k) := O.rshift k ;
+denote_nf (N_rcons i r) := O.rcons i (denote_nf r) ;
+denote_nf (N_rcomp k xr r) := O.rcomp (O.rcomp (O.rshift k) xr) (denote_nf r) ;
+
+denote_nf (N_sshift k) := O.sshift k ;
+denote_nf (N_scons t s) := O.scons (denote_nf t) (denote_nf s) ;
+denote_nf (N_scomp k xs s) := O.scomp (O.scomp (O.sshift k) xs) (denote_nf s) ;
+denote_nf (N_sren r) := fun i => O.E_var (denote_nf r i) ;
+
+denote_nf (@N_rinst_l Kt xt r) := O.rename xt (denote_nf r) ;
+denote_nf (@N_rinst_l (Ka _) xt r) := O.rename xt (denote_nf r) ;
+denote_nf (@N_rinst_l (Kal _) xt r) := O.rename xt (denote_nf r) ;
+
+denote_nf (@N_sinst_l Kt xt s) := O.substitute xt (denote_nf s) ;
+denote_nf (@N_sinst_l (Ka _) xt s) := O.substitute xt (denote_nf s) ;
+denote_nf (@N_sinst_l (Kal _) xt s) := O.substitute xt (denote_nf s) ;
+
+denote_nf (N_rinst_r i xr r) := O.rename (O.E_var i) (O.rcomp xr (denote_nf r)) ;
+denote_nf (N_sinst_r i xs s) := O.substitute (O.E_var i) (O.scomp xs (denote_nf s)).
+
+(*********************************************************************************)
+(** *** Normalization. *)
+(*********************************************************************************)
+
+(** Tail of a normal form renaming. *)
+Equations rtail : nf_ren -> nf_ren := 
+rtail (N_rshift k) := N_rshift (S k) ;
+rtail (N_rcons _ r) := r ;
+rtail (N_rcomp k xr r) := N_rcomp (S k) xr r.
+
+Lemma rtail_sound r : denote_nf (rtail r) =₁ O.rcomp (O.rshift 1) (denote_nf r).
+Proof. 
+funelim (rtail r) ; simp rtail denote_nf.
+- now rewrite O.rshift_succ_l.
+- now rewrite O.rshift_rcons.
+- repeat rewrite <-O.rcomp_assoc. now rewrite O.rshift_succ_l.
+Qed.     
+
+(** Drop the first [k] elements in a normal form renaming. *)
+Equations rdrop : nat -> nf_ren -> nf_ren :=
+rdrop 0 r := r ;
+rdrop (S k) r := rtail (rdrop k r).
+
+Lemma rdrop_sound k r : denote_nf (rdrop k r) =₁ O.rcomp (O.rshift k) (denote_nf r).
+Proof.
+funelim (rdrop k r) ; simp denote_nf.
+- now rewrite O.rcomp_rid_l.
+- rewrite rtail_sound, H. now rewrite <-O.rcomp_assoc, O.rshift_succ_l.
+Qed.  
+
+(** Apply a normal form renaming to a de Bruijn index. *)
+Equations rapply : nf_ren -> nat -> nat :=
+rapply (N_rshift k) i := k + i ;
+rapply (N_rcons i _) 0 := i ;
+rapply (N_rcons _ r) (S i) := rapply r i ;
+rapply (N_rcomp k xr r) i := rapply r (xr (k + i)).
+
+Lemma rapply_sound r i : rapply r i = denote_nf r i.
+Proof. funelim (rapply r i) ; simp denote_nf ; solve [ auto ]. Qed.
+    
+(** Compose two normal form renamings. *)
+Equations rcomp : nf_ren -> nf_ren -> nf_ren :=
+rcomp (N_rshift k) r := rdrop k r ;
+rcomp (N_rcons i r1) r2 := N_rcons (rapply r2 i) (rcomp r1 r2) ;
+rcomp (N_rcomp k xr r1) r2 := N_rcomp k xr (rcomp r1 r2).
+
+Lemma rcomp_sound r1 r2 : 
+  denote_nf (rcomp r1 r2) =₁ O.rcomp (denote_nf r1) (denote_nf r2).
+Proof.
+funelim (rcomp r1 r2) ; simp denote_nf.
+- now rewrite rdrop_sound.
+- now rewrite rapply_sound, O.rcomp_rcons_distrib, H.
+- rewrite H. now repeat rewrite O.rcomp_assoc.
+Qed.
+
+(** Lift a normal form renaming through a binder. *)
+Equations rup : nf_ren -> nf_ren :=
+rup r := N_rcons 0 (rcomp r (N_rshift 1)).
+
+Lemma rup_sound r : denote_nf (rup r) =₁ O.up_ren (denote_nf r).
+Proof. simp rup denote_nf. unfold O.up_ren. now rewrite rcomp_sound. Qed.
+
+(** Instantiate a normal form term with a normal form renaming. *)
+Equations rinst {k} : nf_expr (Km k) -> nf_ren -> nf_expr (Km k) :=
+rinst (N_tvar i) r := N_tvar (rapply r i) ;
+rinst (N_tctor c al) r := N_tctor c (rinst al r) ;
+rinst N_al_nil _ := N_al_nil ;
+rinst (N_al_cons a al) r := N_al_cons (rinst a r) (rinst al r) ;
+rinst (N_abase b x) _ := N_abase b x ;
+rinst (N_aterm t) r := N_aterm (rinst t r) ;
+rinst (N_abind a) r := N_abind (rinst a (rup r)) ;
+rinst (N_rinst_l xt r1) r2 := N_rinst_l xt (rcomp r1 r2) ;
+rinst (N_sinst_l xt s) r := N_sinst_l xt (srcomp s r) ;
+rinst (N_rinst_r i xr r1) r2 := N_rinst_r i xr (rcomp r1 r2) ;
+rinst (N_sinst_r i xs s) r := N_sinst_r i xs (srcomp s r)
+
+(** Compose a normal form substitution with a normal form renaming. *)
+with srcomp : nf_subst -> nf_ren -> nf_subst :=
+srcomp (N_sshift k) r := N_sren (rdrop k r) ;
+srcomp (N_scons t s) r := N_scons (rinst t r) (srcomp s r) ;
+srcomp (N_scomp k xs s) r := N_scomp k xs (srcomp s r) ; 
+srcomp (N_sren r1) r2 := N_sren (rcomp r1 r2).
+
+Lemma rinst_srcomp_sound_aux : 
+  (forall k (t : nf_expr (Km k)) r, 
+    denote_nf (rinst t r) = O.rename (denote_nf t) (denote_nf r)) *
+  (forall s r, 
+    denote_nf (srcomp s r) =₁ fun i => O.rename (denote_nf s i) (denote_nf r)).
+Proof.
+apply rinst_elim with 
+  (P := fun k (t : nf_expr (Km k)) (r : nf_ren) (res : nf_expr (Km k))  => 
+    denote_nf res = O.rename (denote_nf t) (denote_nf r))
+  (P0 := fun (s : nf_subst) (r : nf_ren) (res : nf_subst) =>
+    denote_nf res =₁ fun i => O.rename (denote_nf s i) (denote_nf r)).
+- intros i r. simp denote_nf rename. now rewrite rapply_sound.
+- intros c al r H. simp denote_nf. rewrite H. now simp rename.
+- intros r. now simp denote_nf rename.
+- intros ty tys a al r H1 H2. simp denote_nf rename. now rewrite H1, H2.
+- intros b x r. now simp denote_nf rename.
+- intros t r H. simp denote_nf rename. now rewrite H.
+- intros ty a r H. simp denote_nf rename. now rewrite H, rup_sound.
+- intros k xt r1 r2. destruct k ; simp denote_nf.
+  all: now rewrite rcomp_sound, O.ren_ren.
+- intros k xt s r H. destruct k ; simp denote_nf.
+  all: now rewrite H, O.subst_ren.
+- intros i xr r1 r2. simp denote_nf rename. f_equal. cbv [O.rcomp].
+  now rewrite rcomp_sound.
+- intros i xs s r H. simp denote_nf substitute. cbv [O.scomp]. 
+  now rewrite H, O.subst_ren.
+- intros k r. simp denote_nf. intros i. rewrite rdrop_sound. reflexivity.
+- intros t s r H1 H2. simp denote_nf. rewrite H1, H2. intros [|i] ; reflexivity.
+- intros k xs s r H. simp denote_nf. rewrite H. intros i. cbv [O.scomp O.sshift].
+  simp substitute. now rewrite O.subst_ren.
+- intros r1 r2. simp denote_nf. intros i. simp rename. now rewrite rcomp_sound.
+Qed.
+
+Lemma rinst_sound k (t : nf_expr (Km k)) r :   
+  denote_nf (rinst t r) = O.rename (denote_nf t) (denote_nf r).
+Proof. now apply rinst_srcomp_sound_aux. Qed.
+
+Lemma srcomp_sound s r :
+  denote_nf (srcomp s r) =₁ fun i => O.rename (denote_nf s i) (denote_nf r).
+Proof. now apply rinst_srcomp_sound_aux. Qed.
+
+(** Apply a normal form substitution to a de Bruijn index. *)
+Equations sapply : nf_subst -> nat -> nf_term :=
+sapply (N_sshift k) i := N_tvar (k + i) ;
+sapply (N_scons t _) 0 := t ;
+sapply (N_scons _ s) (S i) := sapply s i ;
+sapply (N_scomp k xs s) i := N_sinst_r (k + i) xs s ;
+sapply (N_sren r) i := N_tvar (rapply r i).  
+
+Lemma sapply_sound s i : denote_nf (sapply s i) = denote_nf s i.
+Proof. 
+funelim (sapply s i) ; simp denote_nf ; try reflexivity.
+- now rewrite H.
+- now rewrite rapply_sound.
+Qed.    
+
+(** Tail of a normal form substitution. *)
+Equations stail : nf_subst -> nf_subst :=
+stail (N_sshift k) := N_sshift (S k) ;
+stail (N_scons t s) := s ;
+stail (N_scomp k xs s) := N_scomp (S k) xs s ;
+stail (N_sren r) := N_sren (rtail r).
+
+Lemma stail_sound s : denote_nf (stail s) =₁ O.scomp (O.sshift 1) (denote_nf s).
+Proof. 
+funelim (stail s) ; simp denote_nf.
+- now rewrite O.sshift_succ_l.
+- now rewrite O.sshift_scons.
+- repeat rewrite <-O.scomp_assoc. now rewrite O.sshift_succ_l.
+- intros i. now rewrite rtail_sound.
+Qed.
+
+(** Drop the first [k] elements in a normal form substitution. *)
+Equations sdrop : nat -> nf_subst -> nf_subst :=
+sdrop 0 s := s ;
+sdrop (S k) s := stail (sdrop k s).
+
+Lemma sdrop_sound k s : denote_nf (sdrop k s) =₁ O.scomp (O.sshift k) (denote_nf s).
+Proof.
+funelim (sdrop k s) ; simp denote_nf.
+- now rewrite O.scomp_sid_l.
+- rewrite stail_sound, H. now rewrite <-O.scomp_assoc, O.sshift_succ_l.
+Qed.  
+
+(** Lift a normal form substitution through a binder. *)
+Equations sup : nf_subst -> nf_subst :=
+sup s := N_scons (N_tvar 0) (srcomp s (N_rshift 1)).
+
+Lemma sup_sound s : denote_nf (sup s) =₁ O.up_subst (denote_nf s).
+Proof. simp sup denote_nf. unfold O.up_subst. now rewrite srcomp_sound. Qed.
+
+(** Compose a normal form renaming with a normal form substitution. *)
+Equations rscomp : nf_ren -> nf_subst -> nf_subst :=
+rscomp (N_rshift k) s := sdrop k s ;
+rscomp (N_rcons i r) s := N_scons (sapply s i) (rscomp r s) ;
+rscomp (N_rcomp k xr r) s := N_scomp k (fun i => O.E_var (xr i)) (rscomp r s).
+
+Lemma rscomp_sound r s : 
+  denote_nf (rscomp r s) =₁ fun i => denote_nf s (denote_nf r i).
+Proof.
+funelim (rscomp r s) ; simp denote_nf.
+- now rewrite sdrop_sound.
+- rewrite sapply_sound, H. intros [|] ; reflexivity.
+- now rewrite H.
+Qed.     
+
+(*(** Size of a normal form expression, not counting [N_sren]. *)
+Equations nf_size {k} : nf_expr k -> nat :=
+nf_size (N_tvar _) := 0 ;
+nf_size (N_tctor _ al) := S (nf_size al) ;
+nf_size N_al_nil := 0 ;
+nf_size (N_al_cons a al) := S (nf_size a + nf_size al) ;
+nf_size (N_abase _ _) := 0 ;
+nf_size (N_aterm t) := S (nf_size t) ;
+nf_size (N_abind a) := S (nf_size a) ;
+
+nf_size (N_rshift _) := 0 ;
+nf_size (N_rcons _ r) := S (nf_size r) ;
+nf_size (N_rcomp _ _ r) := S (nf_size r) ;
+
+nf_size (N_sshift _) := 0 ;
+nf_size (N_scons t s) := S (nf_size t + nf_size s) ;
+nf_size (N_scomp _ _ s) := S (nf_size s) ;
+(** We explicitly don't increase the size when going through [N_sren]. *)
+nf_size (N_sren r) := nf_size r ;
+
+nf_size (N_rinst_l _ r) := S (nf_size r) ;
+nf_size (N_sinst_l _ s) := S (nf_size s) ;
+nf_size (N_rinst_r _ _ r) := S (nf_size r) ;
+nf_size (N_sinst_r _ _ s) := S (nf_size s).*)
+
+(** Instantiate a normal form expression with a normal form substitution. *)
+Equations sinst {k} (t : nf_expr (Km k)) (s : nf_subst) : nf_expr (Km k) by struct t :=
+sinst (N_tvar i) s := sapply s i ;
+sinst (N_tctor c al) s := N_tctor c (sinst al s) ;
+sinst N_al_nil _ := N_al_nil ;
+sinst (N_al_cons a al) s := N_al_cons (sinst a s) (sinst al s) ;
+sinst (N_abase b x) _ := N_abase b x ;
+sinst (N_aterm t) s := N_aterm (sinst t s) ;
+sinst (N_abind a) s := N_abind (sinst a (sup s)) ;
+sinst (N_rinst_l xt r) s := N_sinst_l xt (rscomp r s) ;
+sinst (N_sinst_l xt s1) s2 := N_sinst_l xt (scomp s1 s2) ;
+sinst (N_rinst_r i xr r) s := N_sinst_r i (fun i => O.E_var (xr i)) (rscomp r s) ;
+sinst (N_sinst_r i xs s1) s2 := N_sinst_r i xs (scomp s1 s2)
+
+(** Compose two normal form substitutions. *)
+with scomp (s1 : nf_subst) (s2 : nf_subst) : nf_subst by struct s1 :=
+scomp (N_sshift k) s := sdrop k s ;
+scomp (N_scons t s1) s2 := N_scons (sinst t s1) (scomp s1 s2) ;
+scomp (N_scomp k xs s1) s2 := N_scomp k xs (scomp s1 s2) ; 
+scomp (N_sren r) s := rscomp r s.
+
+Lemma sinst_scomp_sound_aux : 
+  (forall k (t : nf_expr (Km k)) s, 
+    denote_nf (sinst t s) = O.substitute (denote_nf t) (denote_nf s)) *
+  (forall s1 s2, 
+    denote_nf (scomp s1 s2) =₁ O.scomp (denote_nf s1) (denote_nf s2)).
+Proof.
+apply sinst_elim with 
+  (P := fun k (t : nf_expr (Km k)) (s : nf_subst) (res : nf_expr (Km k))  => 
+    denote_nf res = O.substitute (denote_nf t) (denote_nf s))
+  (P0 := fun (s1 s2 res : nf_subst) =>
+    denote_nf res =₁ O.scomp (denote_nf s1) (denote_nf s2)).
+- intros i s. now rewrite sapply_sound.
+- intros c al s H. simp denote_nf. now rewrite H.
+- reflexivity.
+- intros ty tys a al s H1 H2. simp denote_nf substitute. now rewrite H1, H2.
+- intros b x s. now simp denote_nf substitute.
+- intros t s H. simp denote_nf substitute. now rewrite H.
+- intros ty a s H. simp denote_nf substitute. now rewrite H, sup_sound.
+- intros k xt r s. destruct k ; simp denote_nf substitute.
+  all: now rewrite rscomp_sound, O.ren_subst.
+- intros k xt s1 s2 H. destruct k ; simp denote_nf substitute.
+  all: now rewrite H, O.subst_subst.
+- intros i xr r s. simp denote_nf substitute rename.
+  cbv [O.scomp]. simp substitute. now rewrite rscomp_sound.
+- intros i xs s1 s2 H. simp denote_nf substitute. 
+  cbv [O.scomp]. now rewrite H, O.subst_subst.
+- intros k s. simp denote_nf. now rewrite sdrop_sound.
+- intros t s1 s2 H1 H2. simp denote_nf substitute.           
+
+
+    
